src/request_response_authenticated/DY.Example.RequestResponseAuthenticated.Debug.Proof.fst
@@ -1,0 +1,74 @@
+module DY.Example.RequestResponseAuthenticated.Debug.Proof
+
+open DY.Core
+open DY.Lib
+open DY.Example.RequestResponseAuthenticated.Protocol.Total
+open DY.Example.RequestResponseAuthenticated.Protocol.Stateful
+open DY.Example.RequestResponseAuthenticated.Protocol.Stateful.Proof
+open DY.Example.RequestResponseAuthenticated.Debug
+
+/// This module proves that the debug function
+/// fulfills the trace invariants.
+///
+/// The proof works automatically because each
+/// stateful proof as a SMTPat (`[SMTPat (trace_invariant tr); SMTPat (protocol_function)]`).
+/// Another way to do this proof is to basically
+/// duplicate the code from the debug function and
+/// call all the lemmas for the stateful code manually.
+
+#set-options "--fuel 0 --ifuel 5 --z3rlimit 100 --z3cliopt 'smt.qi.eager_threshold=100'"
+val debug_proof:
+  tr:trace ->
+  Lemma
+  (requires
+    trace_invariant tr
+  )
+  (ensures (
+    let (_, tr_out) = debug () tr in
+    trace_invariant tr_out
+    )
+  )
+let debug_proof tr =
+  let (_, tr_out) = debug () tr in
+
+  (* debug_print_string is non-traceful *)
+  let client = "client" in
+  let server = "server" in
+
+  let (x_init, tr_init) = initialize_communication_reqres message_t client server tr
+  in
+  assert(trace_invariant tr_init);
+  match x_init with
+  | None ->
+      assert(tr_init == tr_out)
+  | Some (client_comm_keys_sess_ids, server_comm_keys_sess_ids) ->
+
+      let (x_req, tr_req) =
+        client_send_request
+          client_comm_keys_sess_ids client server tr_init
+      in
+      assert(trace_invariant tr_req);
+      match x_req with
+      | None ->
+          assert(tr_req == tr_out)
+      | Some (sid, msg_id) ->
+
+          let (x_srv, tr_srv) =
+            server_receive_request_send_response
+              server_comm_keys_sess_ids server msg_id tr_req
+          in
+          assert(trace_invariant tr_srv);
+          match x_srv with
+          | None ->
+              assert(tr_srv == tr_out)
+          | Some msg_id ->
+
+              let (x_cli, tr_cli) =
+                client_receive_response client sid msg_id tr_srv
+              in
+              assert(trace_invariant tr_cli);
+              match x_cli with
+              | None ->
+                  assert(tr_cli == tr_out)
+              | Some () ->
+                  assert(tr_cli == tr_out)
