src/request_response_authenticated/DY.Example.RequestResponseAuthenticated.Protocol.Total.Proof.fst
@@ -1,0 +1,51 @@
+module DY.Example.RequestResponseAuthenticated.Protocol.Total.Proof
+
+open Comparse
+open DY.Core
+open DY.Lib
+open DY.Example.RequestResponseAuthenticated.Protocol.Total
+open DY.Example.RequestResponseAuthenticated.Protocol.Stateful
+
+#set-options "--fuel 0 --ifuel 0 --z3cliopt 'smt.qi.eager_threshold=100'"
+
+(*** Cryptographic invariants ***)
+
+val crypto_usages_protocol: crypto_usages
+instance crypto_usages_protocol = default_crypto_usages
+
+val pke_pred_list_protocol: list (string & pke_crypto_predicate)
+let pke_pred_list_protocol = [
+  pke_crypto_predicate_and_tag_communication_layer_reqres message_t;
+]
+
+val sign_pred_list_protocol: list (string & sign_crypto_predicate)
+let sign_pred_list_protocol = [
+  sign_crypto_predicate_and_tag_communication_layer_reqres message_t;
+]
+
+val aead_pred_list_protocol: list (string & aead_crypto_predicate)
+let aead_pred_list_protocol = [
+  aead_crypto_predicate_and_tag_communication_layer_reqres message_t;
+]
+
+#push-options "--ifuel 2 --fuel 0"
+val crypto_predicates_protocol: crypto_predicates
+let crypto_predicates_protocol = {
+  default_crypto_predicates with
+
+  pke_pred = mk_pke_predicate pke_pred_list_protocol;
+
+  sign_pred = mk_sign_predicate sign_pred_list_protocol;
+
+  aead_pred = mk_aead_predicate aead_pred_list_protocol;
+}
+#pop-options
+
+instance crypto_invariants_protocol: crypto_invariants = {
+  usages = crypto_usages_protocol;
+  preds = crypto_predicates_protocol;
+}
+
+let _ = do_split_boilerplate mk_pke_predicate_correct pke_pred_list_protocol
+let _ = do_split_boilerplate mk_sign_predicate_correct sign_pred_list_protocol
+let _ = do_split_boilerplate mk_aead_predicate_correct aead_pred_list_protocol
