src/request_response_authenticated/DY.Example.RequestResponseAuthenticated.Protocol.Total.fst
@@ -1,0 +1,31 @@
+module DY.Example.RequestResponseAuthenticated.Protocol.Total
+
+open Comparse
+open DY.Core
+open DY.Lib
+
+(*
+  Client -> Server: enc{client, nonce}
+  Server -> Client: enc{nonce}
+*)
+
+[@@with_bytes bytes]
+type request = {
+  nonce: bytes;
+}
+
+%splice [ps_request] (gen_parser (`request))
+%splice [ps_request_is_well_formed] (gen_is_well_formed_lemma (`request))
+
+[@@with_bytes bytes]
+type message_t:eqtype =
+  | Request: request -> message_t
+  | Response: bytes -> message_t
+
+%splice [ps_message_t] (gen_parser (`message_t))
+%splice [ps_message_t_is_well_formed] (gen_is_well_formed_lemma (`message_t))
+
+instance comm_layer_reqres_config_protocol: comm_layer_reqres_config message_t = {
+  reqres_tag = "DY.Lib.Communication.Layer.Reqres.Protocol";
+  reqres_ps_a = ps_message_t;
+}
