src/request_response_authenticated/DY.Example.RequestResponseAuthenticated.SecurityProperties.fst
@@ -1,0 +1,47 @@
+module DY.Example.RequestResponseAuthenticated.SecurityProperties
+
+open DY.Core
+open DY.Lib
+
+open DY.Example.RequestResponseAuthenticated.Protocol.Total
+open DY.Example.RequestResponseAuthenticated.Protocol.Stateful
+open DY.Example.RequestResponseAuthenticated.Protocol.Stateful.Proof
+
+#set-options "--fuel 0 --ifuel 0 --z3cliopt 'smt.qi.eager_threshold=100'"
+
+val nonce_secrecy:
+  tr:trace ->
+  client:principal -> server:principal -> cmeta_data:comm_meta_data message_t -> nonce:bytes ->
+  Lemma
+  (requires
+    trace_invariant tr /\
+    attacker_knows tr nonce /\
+    (
+      (exists sid. state_was_set tr client sid (ClientSendRequest {server; cmeta_data; nonce})) \/
+      (exists sid. state_was_set tr server sid (ServerReceiveRequest {client; nonce})) \/
+      (exists sid. state_was_set tr client sid (ClientReceiveResponse {server; cmeta_data; nonce}))
+    )
+  )
+  (ensures
+    is_corrupt tr (principal_label client) \/ is_corrupt tr (principal_label server)
+  )
+let nonce_secrecy tr client server cmeta_data nonce =
+  attacker_only_knows_publishable_values tr nonce
+
+
+#push-options "--fuel 1"
+val server_authentication:
+  tr:trace -> i:timestamp ->
+  client:principal -> response:message_t -> cmeta_data:comm_meta_data message_t ->
+  Lemma
+  (requires
+    trace_invariant tr /\
+    event_triggered_at tr i client (CommClientReceiveResponse client response cmeta_data <: communication_reqres_event message_t)    
+  )
+  (ensures
+    event_triggered (prefix tr i) cmeta_data.server (CommServerSendResponse cmeta_data.client cmeta_data.server cmeta_data.request response cmeta_data.key <: communication_reqres_event message_t) \/
+    is_corrupt (prefix tr i) (principal_label client) \/ 
+    is_corrupt (prefix tr i) (principal_label cmeta_data.server)
+  )
+let server_authentication tr i client response cmeta_data = ()
+#pop-options
